TrueLiveness.v
@@ -1,5 +1,5 @@
 Require Import AllInRel List Map Env DecSolve.
-Require Import IL Annotation AutoIndTac Bisim Exp MoreExp.
+Require Import IL Annotation AutoIndTac Bisim Exp MoreExp SetOperations.
 Require Export Liveness Filter LabelsDefined OUnion.
 
 Set Implicit Arguments.
@@ -15,39 +15,39 @@ Inductive argsLive (Caller Callee:set var) : args -> params -> Prop :=
 
 Lemma argsLive_length lv bv Y Z
   : argsLive lv bv Y Z
-  -> length Y = length Z.
+    -> length Y = length Z.
 Proof.
   intros. general induction H; simpl; eauto.
 Qed.
 
 Lemma argsLive_liveSound lv blv Y Z
-: argsLive lv blv Y Z
-  -> forall (n : nat) (y : exp),
+  : argsLive lv blv Y Z
+    -> forall (n : nat) (y : exp),
       get (filter_by (fun y : var => B[y ∈ blv]) Z Y) n y ->
       live_exp_sound y lv.
 Proof.
-      intros. general induction H; simpl in * |- *.
-      - isabsurd.
-      - decide (z ∈ blv); eauto.
-        inv H1; eauto.
+  intros. general induction H; simpl in * |- *.
+  - isabsurd.
+  - decide (z ∈ blv); eauto.
+    inv H1; eauto.
 Qed.
 
 Lemma argsLive_live_exp_sound lv blv Y Z y z n
-: argsLive lv blv Y Z
-  -> get Y n y
-  -> get Z n z
-  -> z ∈ blv
-  -> live_exp_sound y lv.
+  : argsLive lv blv Y Z
+    -> get Y n y
+    -> get Z n z
+    -> z ∈ blv
+    -> live_exp_sound y lv.
 Proof.
   intros. general induction n; inv H0; inv H1; inv H; intuition; eauto.
 Qed.
 
 Lemma argsLive_agree_on' (V E E':onv val) lv blv Y Z v v'
-:  argsLive lv blv Y Z
- -> agree_on eq lv E E'
- -> omap (exp_eval E) Y = Some v
- -> omap (exp_eval E') Y = Some v'
- -> agree_on eq blv (V [Z <-- List.map Some v]) (V [Z <-- List.map Some v']).
+  :  argsLive lv blv Y Z
+     -> agree_on eq lv E E'
+     -> omap (exp_eval E) Y = Some v
+     -> omap (exp_eval E') Y = Some v'
+     -> agree_on eq blv (V [Z <-- List.map Some v]) (V [Z <-- List.map Some v']).
 Proof.
   intros. general induction H; simpl in * |- *; eauto.
   - monad_inv H2. monad_inv H3.
@@ -60,12 +60,12 @@ Proof.
 Qed.
 
 Lemma argsLive_agree_on (V V' E E':onv val) lv blv Y Z v v'
-: agree_on eq (blv \ of_list Z) V V'
-  -> argsLive lv blv Y Z
-  -> agree_on eq lv E E'
-  -> omap (exp_eval E) Y = Some v
-  -> omap (exp_eval E') Y = Some v'
-  -> agree_on eq blv (V [Z <-- List.map Some v]) (V' [Z <-- List.map Some v']).
+  : agree_on eq (blv \ of_list Z) V V'
+    -> argsLive lv blv Y Z
+    -> agree_on eq lv E E'
+    -> omap (exp_eval E) Y = Some v
+    -> omap (exp_eval E') Y = Some v'
+    -> agree_on eq blv (V [Z <-- List.map Some v]) (V' [Z <-- List.map Some v']).
 Proof.
   intros. etransitivity; eauto using argsLive_agree_on'.
   eapply update_with_list_agree; eauto.
@@ -73,67 +73,86 @@ Proof.
   rewrite map_length; congruence.
 Qed.
 
+Lemma filter_by_incl_argsLive lv blv Y Z
+  : ❬Y❭ = ❬Z❭
+    -> list_union (Exp.freeVars ⊝ filter_by (fun x => if [x \In blv] then true else false) Z Y) ⊆ lv
+    -> argsLive lv blv Y Z.
+Proof.
+  intros LEN INCL. length_equify.
+  general induction LEN; simpl in *; eauto using argsLive.
+  - econstructor.
+    + cases in INCL; try congruence; eauto.
+      * eapply IHLEN. rewrite <- INCL.
+        simpl List.map. rewrite list_union_cons. eauto with cset.
+    + intros. cases in INCL.
+      simpl List.map in INCL.
+      rewrite list_union_cons in INCL.
+      eapply live_exp_sound_incl;[| eapply live_freeVars].
+      rewrite <- INCL. eauto with cset.
+Qed.
+
 Inductive true_live_sound (i:overapproximation)
-  : list ((؟ (set var) * params)) -> stmt -> ann (؟ (set var)) -> Prop :=
-| TLOpr x Lv b lv e al
-  :  true_live_sound i Lv b al
-  -> (x ∈ oget (getAnn al) -> live_exp_sound e lv)
-  -> (oget (getAnn al)\{{x}}) ⊆ lv
-  -> true_live_sound i Lv (stmtLet x e b) (ann1 (Some lv) al)
-| TLIf Lv e b1 b2 lv al1 al2
-  :  true_live_sound i Lv b1 al1
-  -> true_live_sound i Lv b2 al2
-  -> (exp2bool e = None -> live_exp_sound e lv)
-  -> (exp2bool e <> Some false -> oget (getAnn al1) ⊆ lv)
-  -> (exp2bool e <> Some true -> oget (getAnn al2) ⊆ lv)
-  -> true_live_sound i Lv (stmtIf e b1 b2) (ann2 (Some lv) al1 al2)
-| TLGoto l Y Lv lv blv Z
-  : get Lv (counted l) (Some blv,Z)
-  -> (if isImperative i then  (blv \ of_list Z ⊆ lv) else True)
-  -> argsLive lv blv Y Z
-  -> length Y = length Z
-  -> true_live_sound i Lv (stmtApp l Y) (ann0 (Some lv))
-| TLReturn Lv e lv
+  : list params -> list (set var) -> stmt -> ann (set var) -> Prop :=
+| TLOpr ZL Lv x b lv e al
+  :  true_live_sound i ZL Lv b al
+     -> (x ∈ getAnn al -> live_exp_sound e lv)
+     -> (getAnn al\{{x}}) ⊆ lv
+     -> true_live_sound i ZL Lv (stmtLet x e b) (ann1 lv al)
+| TLIf ZL Lv e b1 b2 lv al1 al2
+  :  (exp2bool e <> Some false -> true_live_sound i ZL Lv b1 al1)
+     -> (exp2bool e <> Some true -> true_live_sound i ZL Lv b2 al2)
+     -> (exp2bool e = None -> live_exp_sound e lv)
+     -> (exp2bool e <> Some false -> getAnn al1 ⊆ lv)
+     -> (exp2bool e <> Some true -> getAnn al2 ⊆ lv)
+     -> true_live_sound i ZL Lv (stmtIf e b1 b2) (ann2 lv al1 al2)
+| TLGoto ZL Lv l Y lv blv Z
+  : get ZL (counted l) Z
+    -> get Lv (counted l) blv
+    -> (if isImperative i then  (blv \ of_list Z ⊆ lv) else True)
+    -> argsLive lv blv Y Z
+    -> length Y = length Z
+    -> true_live_sound i ZL Lv (stmtApp l Y) (ann0 lv)
+| TLReturn ZL Lv e lv
   : live_exp_sound e lv
-  -> true_live_sound i Lv (stmtReturn e) (ann0 (Some lv))
-| TLExtern x Lv b lv Y al f
-  : true_live_sound i Lv b al
-  -> (forall n y, get Y n y -> live_exp_sound y lv)
-  -> (oget (getAnn al)\{{x}}) ⊆ lv
-  -> true_live_sound i Lv (stmtExtern x f Y b) (ann1 (Some lv) al)
-| TLLet Lv F t lv als alt Lv'
-  : true_live_sound i (Lv' ++ Lv) t alt
-    -> Lv' = zip pair (getAnn ⊝ als) (fst ⊝ F)
-    -> (forall n x Z, get Lv' n ((Some x), Z) -> trueIsCalled t (LabI n))
+    -> true_live_sound i ZL Lv (stmtReturn e) (ann0 lv)
+| TLExtern ZL Lv x b lv Y al f
+  : true_live_sound i ZL Lv b al
+    -> (forall n y, get Y n y -> live_exp_sound y lv)
+    -> (getAnn al\{{x}}) ⊆ lv
+    -> true_live_sound i ZL Lv (stmtExtern x f Y b) (ann1 lv al)
+| TLLet ZL Lv F t lv als alt
+  : true_live_sound i (fst ⊝ F ++ ZL) (getAnn ⊝ als ++ Lv) t alt
     -> length F = length als
-    -> (forall n Zs a lv, get F n Zs ->
+    -> (forall n Zs a, get F n Zs ->
                  get als n a ->
-                 getAnn a = Some lv ->
-                 true_live_sound i (Lv' ++ Lv) (snd Zs) a)
-    -> (forall n Zs a lv, get F n Zs ->
-                    get als n a ->
-                    getAnn a = Some lv ->
-                    if isFunctional i then (oget (getAnn a) \ of_list (fst Zs)) ⊆ lv else True)
-    -> oget (getAnn alt) ⊆ lv
-    -> true_live_sound i Lv (stmtFun F t)(annF (Some lv) als alt).
+                 true_live_sound i (fst ⊝ F ++ ZL) (getAnn ⊝ als ++ Lv) (snd Zs) a)
+    -> (forall n Zs a, get F n Zs ->
+                 get als n a ->
+                 if isFunctional i then (getAnn a \ of_list (fst Zs)) ⊆ lv
+                 else True)
+    -> getAnn alt ⊆ lv
+    -> true_live_sound i ZL Lv (stmtFun F t)(annF lv als alt).
 
 
-Lemma true_live_sound_overapproximation_I Lv s slv
-: true_live_sound FunctionalAndImperative Lv s slv -> true_live_sound Imperative Lv s slv.
+Lemma true_live_sound_overapproximation_I ZL Lv s slv
+  : true_live_sound FunctionalAndImperative ZL Lv s slv
+    -> true_live_sound Imperative ZL Lv s slv.
 Proof.
   intros. general induction H; simpl in * |- *; econstructor; simpl; eauto.
 Qed.
 
-Lemma true_live_sound_overapproximation_F Lv s slv
-: true_live_sound FunctionalAndImperative Lv s slv -> true_live_sound Functional Lv s slv.
+Lemma true_live_sound_overapproximation_F ZL Lv s slv
+  : true_live_sound FunctionalAndImperative ZL Lv s slv
+    -> true_live_sound Functional ZL Lv s slv.
 Proof.
   intros. general induction H; simpl in * |- *; econstructor; simpl; eauto.
 Qed.
 
+(*
 Lemma true_live_sound_trueIsCalled i Lv s slv l
   : true_live_sound i Lv s slv
     -> trueIsCalled s l
-    -> exists lv Z, get Lv (counted l) (Some lv, Z).
+    -> exists lv Z, get Lv (counted l) (lv, Z).
 Proof.
   intros Live IC. destruct l; simpl in *.
   general induction IC; invt true_live_sound; eauto.
@@ -149,4 +168,4 @@ Proof.
     rewrite zip_length2 in H; eauto with len.
     rewrite map_length in H.
     orewrite (❬F❭ + n - ❬als❭ = n) in H. eauto.
-Qed.
+Qed.*)
