LivenessAnalysisCorrect.v
@@ -1,0 +1,130 @@
+Require Import CSet Le Var.
+
+Require Import Plus Util AllInRel Map CSet.
+Require Import Val Var Env EnvTy IL Annotation Lattice DecSolve Analysis Filter Terminating.
+Require Import Analysis LivenessAnalysis TrueLiveness Subterm.
+
+Set Implicit Arguments.
+
+Instance proj1_eq_sym X `{OrderedType X} (U:set X)
+  : Symmetric (fun x y : {s0 : ⦃X⦄ | s0 ⊆ U} => proj1_sig x [=] proj1_sig y).
+Proof.
+  hnf; intros [x ?] [y ?]; simpl; intros; symmetry; eauto.
+Qed.
+
+Instance proj1_eq_transitive X `{OrderedType X} (U:set X)
+  : Transitive (fun x y : {s0 : ⦃X⦄ | s0 ⊆ U} => proj1_sig x [=] proj1_sig y).
+Proof.
+  hnf; intros [x ?] [y ?] [z ?]; simpl; intros; etransitivity; eauto.
+Qed.
+
+Definition liveness_analysis_correct sT ZL LV s a (ST:subTerm s sT)
+  : ann_R
+         (fun x y : {s0 : ⦃var⦄ | s0 ⊆ occurVars sT} => proj1_sig x [=] proj1_sig y)
+         (backward (fun s : stmt => {x : ⦃var⦄ | x ⊆ occurVars s})
+                   liveness_transform_dep ZL LV ST a) a
+    -> annotation s a
+    -> labelsDefined s (length ZL)
+    -> labelsDefined s (length LV)
+    -> paramsMatch s (@length _ ⊝ ZL)
+    -> true_live_sound Imperative ZL (@proj1_sig _ _ ⊝ LV) s
+                      (mapAnn (@proj1_sig _ _) a).
+Proof.
+  intros EQ Ann DefZL DefLV PM.
+  general induction Ann; simpl in *; inv DefZL; inv DefLV; inv PM.
+  - inv EQ.
+    pose proof (ann_R_get H7); simpl in *.
+    econstructor.
+    eapply IHAnn; eauto.
+    + intros. destruct a. simpl in *.
+      rewrite getAnn_mapAnn in H0.
+      rewrite <- H in H0.
+      cases in H2.
+      eapply live_exp_sound_incl; [| eapply live_freeVars].
+      rewrite <- H2. eapply incl_right.
+    + rewrite <- H2.
+      simpl. rewrite getAnn_mapAnn.
+      eapply incl_union_left.
+      rewrite H. cset_tac.
+  - inv EQ.
+    simpl in *.
+    econstructor; intros.
+    + eapply IHAnn1; eauto.
+    + eapply IHAnn2; eauto.
+    + repeat cases in H9; try congruence.
+      eapply live_exp_sound_incl; [| eapply live_freeVars].
+      rewrite <- H9. eauto with cset.
+    + rewrite getAnn_mapAnn.
+      rewrite <- H9.
+      eapply ann_R_get in H12. rewrite <- H12.
+      cases. reflexivity.
+      cases. congruence. eauto with cset.
+    + rewrite getAnn_mapAnn.
+      rewrite <- H9. cases. congruence.
+      eapply ann_R_get in H13. rewrite <- H13.
+      cases. reflexivity. eauto with cset.
+  - inv EQ. simpl in *.
+    edestruct (get_in_range _ H2) as [Z ?]; eauto.
+    edestruct (get_in_range _ H3) as [[Lv ?] ?]; eauto.
+    econstructor; eauto.
+    + simpl. rewrite <- H4.
+      repeat erewrite get_nth; eauto.
+      eapply incl_left.
+    + simpl in *.
+      erewrite get_nth in H4; eauto using map_get_1.
+      erewrite get_nth in H4; eauto. simpl in *.
+      eapply filter_by_incl_argsLive; eauto.
+      inv_get; eauto.
+      rewrite <- H4; eauto with cset.
+    + inv_get; eauto.
+  - inv EQ. econstructor.
+    simpl in *. rewrite <- H1. eapply live_freeVars.
+  - inv EQ. simpl in *.
+    econstructor.
+    eapply IHAnn; eauto.
+    + intros.
+      eapply live_exp_sound_incl; [|eapply live_freeVars].
+      rewrite <- H2. eapply incl_union_right.
+      eapply incl_list_union; eauto using map_get_1.
+    + rewrite getAnn_mapAnn. rewrite <- H2.
+      eapply ann_R_get in H7. rewrite <- H7.
+      eauto with cset.
+  - inv EQ.
+    simpl in *.
+    econstructor.
+    + rewrite map_map.
+      erewrite map_ext with (l:=sa);[| intros; rewrite getAnn_mapAnn; reflexivity].
+      rewrite <- map_map with (l:=sa). rewrite <- map_app.
+      eapply (IHAnn (fst ⊝ s ++ ZL) (getAnn ⊝ sa ++ LV)
+             (subTerm_EQ_Fun1 eq_refl ST)); eauto.
+      etransitivity; eauto.
+      eapply (@backward_ext sT (fun s => { x : ⦃var⦄ | x ⊆ occurVars s}) _
+                            (liveness_transform_dep)
+                            (@liveness_transform_dep_ext sT)); eauto.
+      eapply PIR2_app; eauto.
+      eapply PIR2_get; eauto with len.
+      intros; inv_get.
+      exploit H16; eauto.
+      eapply ann_R_get in H9. symmetry; eauto.
+      * rewrite app_length, map_length. eauto.
+      * rewrite app_length, map_length, <- H. eauto.
+      * rewrite map_app.
+        rewrite map_map. eauto.
+    + rewrite map_length. eauto.
+    + intros. inv_get.
+      rewrite map_map.
+      erewrite map_ext with (l:=sa);[| intros; rewrite getAnn_mapAnn; reflexivity].
+      rewrite <- map_map with (l:=sa). rewrite <- map_app.
+      edestruct (@get_backwardF sT _ (backward (fun s0 : stmt => {x1 : ⦃var⦄ | x1 ⊆ occurVars s0}) liveness_transform_dep)); eauto.
+      eapply (H1 _ _ _ H3 H2 (fst ⊝ s ++ ZL) (getAnn ⊝ sa ++ LV)
+             x0); eauto.
+      * rewrite app_length, map_length. eauto.
+      * rewrite app_length, map_length, <- H. eauto.
+      * rewrite map_app. exploit H6; eauto.
+        rewrite map_map. eauto.
+    + intros. inv_get. simpl. eauto.
+    + rewrite getAnn_mapAnn.
+      eapply ann_R_get in H17.
+      rewrite <- H17.
+      rewrite <- H13. reflexivity.
+Qed.
